

1. $12345678_{10} \rightarrow X_{16}$

Решение:

Делим на 16

$$12345678 : 16 = 771604 \text{ (остаток 14)}$$

$$771604 : 16 = 48225 \text{ (остаток 4)}$$

$$48225 : 16 = 3014 \text{ (остаток 1)}$$

$$3014 : 16 = 188 \text{ (остаток 16)}$$

$$188 : 16 = 11 \text{ (остаток 13)}$$

$$11 : 16 = 0 \text{ (остаток 11)}$$

Ответ: BCG14E

$1000000_{10} \rightarrow X_{16}$

$$1000000 : 16 = 62500 \text{ (остаток 0)}$$

$$62500 : 16 = 3906 \text{ (остаток 4)}$$

$$3906 : 16 = 244 \text{ (остаток 2)}$$

$$244 : 16 = 15 \text{ (остаток 4)}$$

$$15 : 16 = 0 \text{ (остаток 15)}$$

Ответ: E4240

$$2. \quad 12345678_{16} \rightarrow X_{10}$$

Решение:

$$8 \cdot 16^0 = 8 \cdot 1 = 8$$

$$7 \cdot 16^1 = 7 \cdot 16 = 112$$

$$6 \cdot 16^2 = 6 \cdot 256 = 1536$$

$$5 \cdot 16^3 = 5 \cdot 4096 = 20480$$

$$4 \cdot 16^4 = 4 \cdot 65536 = 262144$$

$$3 \cdot 16^5 = 3 \cdot 1048576 = 3145728$$

$$2 \cdot 16^6 = 2 \cdot 16777216 = 33554432$$

$$1 \cdot 16^7 = 1 \cdot 268435456 = 268435456$$

$$\text{Ответ: } 305419896$$

$$1000000_{16} \rightarrow X_{10}$$

$$0 \cdot 16^0 = 0$$

$$0 \cdot 16^1 = 0$$

$$0 \cdot 16^2 = 0$$

$$0 \cdot 16^3 = 0$$

$$0 \cdot 16^4 = 0$$

$$0 \cdot 16^5 = 0$$

$$1 \cdot 16^6 = 16777216$$

$$\text{Ответ: } 16777216$$

3. Сгущённого молока (A) и мёда (B) и
можно без хлеба (C)

$$A \&\& B \&\& !C$$

4. Докажите тождества:

$$A \rightarrow B = !A \vee B$$

Таблица истинности для $A \rightarrow B$ и $!A \vee B$

A	B	$A \rightarrow B$	$!A$	$!A \vee B$
0	0	1	1	1
0	1	1	1	1
1	0	0	0	0
1	1	1	0	1

$\curvearrowright = \curvearrowleft$

Таблица истинности для $A \leftrightarrow B$ и
 $(A \&\& B) \vee (!A \&\& !B)$

A	B	$A \leftrightarrow B$	$(A \&\& B) \vee (!A \&\& !B)$
0	0	1	1
0	1	0	0
1	0	0	0
1	1	1	1

$\curvearrowright = \curvearrowleft$

6. Упростите выражение.

$$X = (B \rightarrow A) \cdot (\overline{A+B}) (A \rightarrow C)$$

$$(\overline{A+B}) = A' \cdot B'$$

$$X = (B \rightarrow A) \cdot A' \cdot B' \cdot (A \rightarrow C)$$

$$B \rightarrow A = B' + A$$

$$A \rightarrow C = A' + C$$

$$X = (B' + A) \cdot (A' \cdot B') \cdot (A' + C)$$

$$(B' + A) \cdot A' = B' \cdot A' + A \cdot A' = B' \cdot A' + 0 = B' \cdot A'$$

$$B' \cdot A' \cdot B' = A' \cdot B'$$

$$X = A' \cdot B' \cdot (A' + C) = A' \cdot B' \cdot A' + A' \cdot B' \cdot C =$$

$$= A' \cdot B' + A' \cdot B' \cdot C = A' \cdot B' (1 + C)$$

$$1 + C = 1$$

$$\boxed{X = A' \cdot B'}$$